Flow/TIP/Big/Correspondence/Located.lean
@@ -1,0 +1,199 @@
+import Flow.TIP.Eval
+import Flow.TIP.Big.CFG
+import Flow.TIP.Big.Correspondence.Refinement
+
+namespace Flow.Eval.Big.Located
+
+open Flow.Eval.Big.Refinement
+open BigCFGBuilder
+
+mutual
+inductive LocatedAt (g : BigCFG) : BigNodeID -> CEK -> Prop where
+| at_skip {n E K} :
+    g.nodeKind n = some (.SEntry .Skip) ->
+    KontMatches g K n E ->
+    LocatedAt g n ⟨.inl .Skip, E, K⟩
+| at_assign {n m x e K E} :
+    g.nodeKind n = some (.SEntry (.Assign x e)) ->
+    g.hasEdge n m .Normal ->
+    LocatedAt g m ⟨.inr e, E, .AssignK x :: K⟩ ->
+    KontMatches g K n E ->
+    LocatedAt g n ⟨.inl (.Assign x e), E, K⟩
+| at_declare {n m x e K E} :
+    g.nodeKind n = some (.SEntry (.Decl x e)) ->
+    g.hasEdge n m .Normal ->
+    LocatedAt g m ⟨.inr e, E, .DeclK x :: K⟩ ->
+    KontMatches g K n E ->
+    LocatedAt g n ⟨.inl (.Decl x e), E, K⟩
+| at_if {n m c t e K E} :
+    g.nodeKind n = some (.SEntry (.If c t e)) ->
+    g.hasEdge n m .Normal ->
+    g.nodeKind m = some (.EEntry c) ->
+    KontMatches g K n E ->
+    LocatedAt g n ⟨.inl (.If c t e), E, K⟩
+| at_while {n m c b K E} :
+    g.nodeKind n = some (.SEntry (.While c b)) ->
+    g.hasEdge n m .Normal ->
+    g.nodeKind m = some (.EEntry c) ->
+    KontMatches g K n E ->
+    LocatedAt g n ⟨.inl (.While c b), E, K⟩
+| at_seq {n s₁ s₂ K E} :
+    LocatedAt g n ⟨.inl s₁, E, .SeqK s₂ :: K⟩ ->
+    LocatedAt g n ⟨.inl (.Seq s₁ s₂), E, K⟩
+| at_sexit {n K E} :
+    g.nodeKind n = some (.SExit) ->
+    KontMatches g K n E ->
+    LocatedAt g n ⟨.inl .Skip, E, K⟩
+| at_expr {n m e E K} :
+    g.nodeKind n = some (.EEntry e) ->
+    g.hasEdge n m .Normal ->
+    g.nodeKind m = some (.EExit) ->
+    KontMatches g K n E ->
+    KontMatches g K m E ->
+    LocatedAt g n ⟨.inr e, E, K⟩
+| at_eexit {n K E v} :
+    g.nodeKind n = some (.EExit) ->
+    KontMatches g K n E ->
+    LocatedAt g n ⟨.inr (.Int v), E, K⟩
+
+-- continuation matches current state
+inductive KontMatches (g : BigCFG) : List Cont -> NodeID -> State -> Prop where
+  | nil {n E} : KontMatches g [] n E
+  | seqK {n m s₂ E K} :
+      g.hasEdge n m .Normal ->
+      LocatedAt g m ⟨.inl s₂, E, K⟩ ->
+      KontMatches g (.SeqK s₂ :: K) n E
+  | assignK {n m x v E K} :
+      g.hasEdge n m .Normal ->
+      g.nodeKind m = some (.SEntry .Skip) ->
+      KontMatches g K m (E.updated x v) ->
+      KontMatches g (.AssignK x :: K) n E
+  | declK {n m x v E K} :
+      g.hasEdge n m .Normal ->
+      g.nodeKind m = some (.SEntry .Skip) ->
+      KontMatches g K m (E.updated x v) ->
+      KontMatches g (.DeclK x :: K) n E
+  | ifKT {n t nT E K f} :
+      g.hasEdge n nT .TBranch ->
+      LocatedAt g nT ⟨.inl t, E, K⟩ ->
+      KontMatches g (.IfK t f :: K) n E
+  | ifKF {n t nF E K f} :
+      g.hasEdge n nF .TBranch ->
+      LocatedAt g nF ⟨.inl f, E, K⟩ ->
+      KontMatches g (.IfK t f :: K) n E
+  | whileKT {n nT c b E K} :
+      g.hasEdge n nT .TBranch ->
+      LocatedAt g nT ⟨.inl b, E, .WhileBackK c b :: K⟩ ->
+      KontMatches g (.WhileK c b :: K) n E
+  | whileKF {n nF c b E K} :
+      g.hasEdge n nF .FBranch ->
+      LocatedAt g nF ⟨.inl b, E, .WhileBackK c b :: K⟩ ->
+      KontMatches g (.WhileK c b :: K) n E
+  | whileBackK {n nc c b E K} :
+      g.hasEdge n nc .Normal ->
+      LocatedAt g nc ⟨.inl (.While c b), E, K⟩ ->
+      KontMatches g (.WhileBackK c b :: K) n E
+  | skipBridge {n m E K} :
+      g.nodeKind n = some (.SEntry .Skip) ->
+      g.nodeKind m = some (.SEntry .Skip) ->
+      g.hasEdge n m .Normal ->
+      KontMatches g K m E ->
+      KontMatches g K n E
+  | binOpLK {n o ne₂ e₂ E K} :
+      g.hasEdge n ne₂ .Normal ->
+      KontMatches g K ne₂ E ->
+      KontMatches g (.BinOpLK o e₂ :: K) n E
+  | binOpRK {n v o nex E K} :
+      g.hasEdge n nex .Normal ->
+      KontMatches g K nex E ->
+      KontMatches g (.BinOpRK v o :: K) n E
+end
+
+private lemma nodeKind_lt {g : BigCFG} {n k}
+    (h : g.nodeKind n = some k) : n < g.nodes.length := by
+  unfold BigCFG.nodeKind at h; grind
+
+theorem LocatedAt.bound {g : BigCFG} {n σ}
+    (h : LocatedAt g n σ) : n < g.nodes.length := by
+  induction h using LocatedAt.rec (motive_2 := fun _ _ _ _ => True) <;>
+    first
+    | trivial
+    | (expose_names; exact nodeKind_lt h) -- ew
+
+theorem step_decorate {g : BigCFG} {n : BigNodeID} {σ σ' : CEK}
+    (hloc : LocatedAt g n σ) (hstep : Step σ σ') :
+    ∃ (n' : NodeID) (h : n < g.nodes.length) (h' : n' < g.nodes.length),
+      BigStepsN g h σ h' σ' ∧ LocatedAt g n' σ' := by
+  have hn := hloc.bound
+  cases hstep with
+  | @SeqEnter s₁ s₂ E K =>
+    cases hloc
+    case _ hloc =>
+    refine ⟨n, hn, hn, ?_, hloc⟩
+    apply BigStepsN.single
+    grind [BigStepN.stutter, Step.SeqEnter]
+  | @SeqMid s₁ s₂ E =>
+    cases hloc with
+    | at_skip hk hmatch =>
+      cases hmatch with
+      | seqK hedge hloc' =>
+        refine ⟨_, hn, hloc'.bound, ?_, ?_⟩
+        · apply BigStepsN.single
+          grind [BigStepN.advance, Step.SeqMid]
+        · exact hloc'
+      | @skipBridge _ m _ _ hk' hk'' hedge ih =>
+        refine ⟨m, hn, nodeKind_lt hk'', ?_, ?_⟩
+        · sorry
+        · sorry
+    | at_sexit =>
+      sorry
+  | @Decl x e E K =>
+    cases hloc
+    case _ m he hk hmatch hloc =>
+    cases hloc with
+    | at_expr hm hmatch' =>
+      have := nodeKind_lt hm
+      refine ⟨m, hn, this, ?_, ?_⟩
+      · apply BigStepsN.single
+        grind [BigStepN.advance, Step.Decl]
+      · constructor <;> assumption
+    | @at_eexit _ _ _ v hm hmatch =>
+      have := nodeKind_lt hm
+      refine ⟨m, hn, this, ?_, ?_⟩
+      · apply BigStepsN.single
+        grind [BigStepN.advance, Step.Decl]
+      · exact LocatedAt.at_eexit hm hmatch
+  | @Assign x e E K =>
+    cases hloc
+    case _ m hedge hk hmatch hloc =>
+    cases hloc with
+    | @at_expr _ m' _ _ _ hm he hm' hmatch' hmatch'' =>
+      have := nodeKind_lt hm
+      refine ⟨m, hn, this, ?_, ?_⟩
+      · apply BigStepsN.single
+        grind [BigStepN.advance, Step.Assign]
+      · exact LocatedAt.at_expr hm he hm' hmatch' hmatch''
+    | @at_eexit _ _ _ v hm hmatch =>
+      have := nodeKind_lt hm
+      refine ⟨m, hn, this, ?_, ?_⟩
+      · apply BigStepsN.single
+        grind [BigStepN.advance, Step.Assign]
+      · exact LocatedAt.at_eexit hm hmatch
+  | @DeclD v E x K =>
+    sorry
+  | @AssignD v E x K =>
+    sorry
+  | @Var E x K v henv =>
+    cases hloc
+    case at_expr m hm he hk hmatch hmatch' =>
+    have := nodeKind_lt hm
+    refine ⟨m, hn, this, ?_, ?_⟩
+    · apply BigStepsN.single
+      grind [BigStepN.advance, Step.Var]
+    · exact LocatedAt.at_eexit hm hmatch
+  | _ => sorry
+
+
+
+
+end Flow.Eval.Big.Located
